KAT/KAT_rKAT_rVCs_ndfun.thy
@@ -502,10 +502,10 @@ proof(subst ndfun_kat_H, simp add: g_orbital_eq p2ndf_def g_ode_def, clarsimp)
 qed
 *)
 
-abbreviation g_global_ode ::"(('a::banach)\<Rightarrow>'a) \<Rightarrow> 'a pred \<Rightarrow> 'a nd_fun" ("(1x\<acute>=_ & _)") 
+abbreviation g_global_ode ::"(('a::banach)\<Rightarrow>'a) \<Rightarrow> 'a upred \<Rightarrow> 'a nd_fun" ("(1x\<acute>=_ & _)") 
   where "(x\<acute>= f & G) \<equiv> (x\<acute>= f & G on UNIV UNIV @ 0)"
 
-abbreviation g_global_ode_inv :: "(('a::banach)\<Rightarrow>'a) \<Rightarrow> 'a pred \<Rightarrow> 'a pred \<Rightarrow> 'a nd_fun" 
+abbreviation g_global_ode_inv :: "(('a::banach)\<Rightarrow>'a) \<Rightarrow> 'a upred \<Rightarrow> 'a upred \<Rightarrow> 'a nd_fun" 
   ("(1x\<acute>=_ & _ DINV _)") where "(x\<acute>= f & G DINV I) \<equiv> (x\<acute>= f & G on UNIV UNIV @ 0 DINV I)"
 
 
